Reworked constraints for Odiv/Odivu for ARM
The instructions should only have the constraints on argument and
result registers if no hardware division is available.  In this case,
floating point caller save registers must be marked as destroyed by
Odiv/Odivu.

arm/AsmToJSON.ml
@@ -278,7 +278,7 @@ let pp_instructions pp ic =
     | Prsc(r1, r2, so) -> instruction pp "Prsc" [Ireg r1; Ireg r2; Shift so]
     | Psbc(r1, r2, so) -> instruction pp "Psbc" [Ireg r1; Ireg r2; Shift so]
     | Psbfx(r1, r2, lsb, sz) -> instruction pp "Psbfx" [Ireg r1; Ireg r2; Long lsb; Long sz]
-    | Psdiv -> instruction pp "Psdiv" [Ireg IR0; Ireg IR0; Ireg IR1]
+    | Psdiv (r1, r2, r3) -> instruction pp "Psdiv" [Ireg r1; Ireg r2; Ireg r3]
     | Psmull(r1, r2, r3, r4) -> instruction pp "Psmull" [Ireg r1; Ireg r2; Ireg r3; Ireg r4]
     | Pstr(r1, r2, so) | Pstr_a(r1, r2, so) -> instruction pp "Pstr" [Ireg r1; Ireg r2; Shift so]
     | Pstr_p(r1, r2, so) -> instruction pp "Pstr_p" [Ireg r1; Ireg r2; Shift so]
@@ -288,7 +288,7 @@ let pp_instructions pp ic =
     | Pstrh_p(r1, r2, so) -> instruction pp "Pstrh_p" [Ireg r1; Ireg r2; Shift so]
     | Psub(r1, r2, so) -> instruction pp "Psub" [Ireg r1; Ireg r2; Shift so]
     | Psubs(r1, r2, so) -> instruction pp "Psubs" [Ireg r1; Ireg r2; Shift so]
-    | Pudiv -> instruction pp "Pudiv" [Ireg IR0; Ireg IR0; Ireg IR1]
+    | Pudiv (r1, r2, r3) -> instruction pp "Pudiv" [Ireg r1; Ireg r2; Ireg r3]
     | Pumull(r1, r2, r3, r4) -> instruction pp "Pumull" [Ireg r1; Ireg r2; Ireg r3; Ireg r4]
     (* Fixup instructions for calling conventions *)
     | Pfcpy_fs(r1, r2) -> instruction pp "Pfcpy_fs" [SFreg r1; SPreg r2]
