arm/extractionMachdep.v
@@ -36,3 +36,10 @@ Extract Constant Archi.big_endian =>
 (* Whether the model is ARMv6T2 or above and hence supports Thumb2. *)
 Extract Constant Archi.thumb2_support =>
   "(Configuration.model = ""armv6t2"" || Configuration.model >= ""armv7"")".
+
+(* Whether the model has hardware supports sdiv and udiv *)
+Extract Constant Archi.hardware_idiv =>
+  "fun () -> begin match  Configuration.model with
+   | ""armv7r"" | ""armv7m"" -> !Clflags.option_mthumb
+   | _ -> false
+   end".
